theories/ssr/ssreflect.v
@@ -1,0 +1,656 @@
+(************************************************************************)
+(*         *   The Coq Proof Assistant / The Coq Development Team       *)
+(*  v      *   INRIA, CNRS and contributors - Copyright 1999-2019       *)
+(* <O___,, *       (see CREDITS file for the list of authors)           *)
+(*   \VV/  **************************************************************)
+(*    //   *    This file is distributed under the terms of the         *)
+(*         *     GNU Lesser General Public License Version 2.1          *)
+(*         *     (see LICENSE file for the text of the license)         *)
+(************************************************************************)
+
+(* This file is (C) Copyright 2006-2015 Microsoft Corporation and Inria. *)
+
+(** #<style> .doc { font-family: monospace; white-space: pre; } </style># **)
+
+Require Import Bool. (* For bool_scope delimiter 'bool'. *)
+Require Import ssrmatching.
+Declare ML Module "ssreflect_plugin".
+
+
+(**
+ This file is the Gallina part of the ssreflect plugin implementation.
+ Files that use the ssreflect plugin should always Require ssreflect and
+ either Import ssreflect or Import ssreflect.SsrSyntax.
+   Part of the contents of this file is technical and will only interest
+ advanced developers; in addition the following are defined:
+   #[#the str of v by f#]# == the Canonical s : str such that f s = v.
+        #[#the str of v#]# == the Canonical s : str that coerces to v.
+        argumentType c == the T such that c : forall x : T, P x.
+          returnType c == the R such that c : T -> R.
+     {type of c for s} == P s where c : forall x : T, P x.
+           nonPropType == an interface for non-Prop Types: a nonPropType coerces
+                          to a Type, and only types that do _not_ have sort
+                          Prop are canonical nonPropType instances. This is
+                          useful for applied views (see mid-file comment).
+             notProp T == the nonPropType instance for type T.
+           phantom T v == singleton type with inhabitant Phantom T v.
+               phant T == singleton type with inhabitant Phant v.
+                 =^~ r == the converse of rewriting rule r (e.g., in a
+                          rewrite multirule).
+             unkeyed t == t, but treated as an unkeyed matching pattern by
+                          the ssreflect matching algorithm.
+             nosimpl t == t, but on the right-hand side of Definition C :=
+                          nosimpl disables expansion of C by /=.
+              locked t == t, but locked t is not convertible to t.
+       locked_with k t == t, but not convertible to t or locked_with k' t
+                          unless k = k' (with k : unit). Coq type-checking
+                          will be much more efficient if locked_with with a
+                          bespoke k is used for sealed definitions.
+          unlockable v == interface for sealed constant definitions of v.
+        Unlockable def == the unlockable that registers def : C = v.
+     #[#unlockable of C#]# == a clone for C of the canonical unlockable for the
+                          definition of C (e.g., if it uses locked_with).
+    #[#unlockable fun C#]# == #[#unlockable of C#]# with the expansion forced to be
+                          an explicit lambda expression.
+  -> The usage pattern for ADT operations is:
+       Definition foo_def x1 .. xn := big_foo_expression.
+       Fact foo_key : unit. Proof. by #[# #]#. Qed.
+       Definition foo := locked_with foo_key foo_def.
+       Canonical foo_unlockable := #[#unlockable fun foo#]#.
+     This minimizes the comparison overhead for foo, while still allowing
+     rewrite unlock to expose big_foo_expression.
+ More information about these definitions and their use can be found in the
+ ssreflect manual, and in specific comments below.                           **)
+
+Set Implicit Arguments.
+Unset Strict Implicit.
+Unset Printing Implicit Defensive.
+
+Module SsrSyntax.
+
+(**
+ Declare Ssr keywords: 'is' 'of' '//' '/=' and '//='. We also declare the
+ parsing level 8, as a workaround for a notation grammar factoring problem.
+ Arguments of application-style notations (at level 10) should be declared
+ at level 8 rather than 9 or the camlp5 grammar will not factor properly.    **)
+
+Reserved Notation "(* x 'is' y 'of' z 'isn't' // /= //= *)" (at level 8).
+Reserved Notation "(* 69 *)" (at level 69).
+
+(**  Non ambiguous keyword to check if the SsrSyntax module is imported  **)
+Reserved Notation "(* Use to test if 'SsrSyntax_is_Imported' *)" (at level 8).
+
+Reserved Notation "<hidden n >" (at level 0, n at level 0,
+  format "<hidden  n >").
+Reserved Notation "T (* n *)" (at level 200, format "T  (* n *)").
+
+End SsrSyntax.
+
+Export SsrMatchingSyntax.
+Export SsrSyntax.
+
+(** Save primitive notation that will be overloaded. **)
+Local Notation CoqGenericIf c vT vF := (if c then vT else vF) (only parsing).
+Local Notation CoqGenericDependentIf c x R vT vF :=
+  (if c as x return R then vT else vF) (only parsing).
+Local Notation CoqCast x T := (x : T) (only parsing).
+
+(** Reserve notation that introduced in this file. **)
+Reserved Notation "'if' c 'then' vT 'else' vF" (at level 200,
+  c, vT, vF at level 200).
+Reserved Notation "'if' c 'return' R 'then' vT 'else' vF" (at level 200,
+  c, R, vT, vF at level 200).
+Reserved Notation "'if' c 'as' x 'return' R 'then' vT 'else' vF" (at level 200,
+  c, R, vT, vF at level 200, x ident).
+
+Reserved Notation "x : T" (at level 100, right associativity,
+  format "'[hv' x '/ '  :  T ']'").
+Reserved Notation "T : 'Type'" (at level 100, format "T  :  'Type'").
+Reserved Notation "P : 'Prop'" (at level 100, format "P  :  'Prop'").
+
+Reserved Notation "[ 'the' sT 'of' v 'by' f ]" (at level 0,
+  format "[ 'the'  sT  'of'  v  'by'  f ]").
+Reserved Notation "[ 'the' sT 'of' v ]" (at level 0,
+  format "[ 'the'  sT  'of'  v ]").
+Reserved Notation "{ 'type' 'of' c 'for' s }" (at level 0,
+  format "{ 'type'  'of'  c  'for'  s }").
+
+Reserved Notation "=^~ r" (at level 100, format "=^~  r").
+
+Reserved Notation "[ 'unlockable' 'of' C ]" (at level 0,
+  format "[ 'unlockable'  'of'  C ]").
+Reserved Notation "[ 'unlockable' 'fun' C ]" (at level 0,
+  format "[ 'unlockable'  'fun'  C ]").
+
+(**
+ To define notations for tactic in intro patterns.
+ When "=> /t" is parsed, "t:%ssripat" is actually interpreted. **)
+Declare Scope ssripat_scope.
+Delimit Scope ssripat_scope with ssripat.
+
+(**
+ Make the general "if" into a notation, so that we can override it below.
+ The notations are "only parsing" because the Coq decompiler will not
+ recognize the expansion of the boolean if; using the default printer
+ avoids a spurious trailing %%GEN_IF. **)
+
+Declare Scope general_if_scope.
+Delimit Scope general_if_scope with GEN_IF.
+
+Notation "'if' c 'then' vT 'else' vF" :=
+  (CoqGenericIf c vT vF) (only parsing) : general_if_scope.
+
+Notation "'if' c 'return' R 'then' vT 'else' vF" :=
+  (CoqGenericDependentIf c c R vT vF) (only parsing) : general_if_scope.
+
+Notation "'if' c 'as' x 'return' R 'then' vT 'else' vF" :=
+  (CoqGenericDependentIf c x R vT vF) (only parsing) : general_if_scope.
+
+(**  Force boolean interpretation of simple if expressions.  **)
+
+Declare Scope boolean_if_scope.
+Delimit Scope boolean_if_scope with BOOL_IF.
+
+Notation "'if' c 'return' R 'then' vT 'else' vF" :=
+  (if c is true as c in bool return R then vT else vF) : boolean_if_scope.
+
+Notation "'if' c 'then' vT 'else' vF" :=
+  (if c%bool is true as _ in bool return _ then vT else vF) : boolean_if_scope.
+
+Notation "'if' c 'as' x 'return' R 'then' vT 'else' vF" :=
+  (if c%bool is true as x in bool return R then vT else vF) : boolean_if_scope.
+
+Open Scope boolean_if_scope.
+
+(**
+ To allow a wider variety of notations without reserving a large number of
+ of identifiers, the ssreflect library systematically uses "forms" to
+ enclose complex mixfix syntax. A "form" is simply a mixfix expression
+ enclosed in square brackets and introduced by a keyword:
+      #[#keyword ... #]#
+ Because the keyword follows a bracket it does not need to be reserved.
+ Non-ssreflect libraries that do not respect the form syntax (e.g., the Coq
+ Lists library) should be loaded before ssreflect so that their notations
+ do not mask all ssreflect forms.                                            **)
+Declare Scope form_scope.
+Delimit Scope form_scope with FORM.
+Open Scope form_scope.
+
+(**
+ Allow overloading of the cast (x : T) syntax, put whitespace around the
+ ":" symbol to avoid lexical clashes (and for consistency with the parsing
+ precedence of the notation, which binds less tightly than application),
+ and put printing boxes that print the type of a long definition on a
+ separate line rather than force-fit it at the right margin.                 **)
+Notation "x : T" := (CoqCast x T) : core_scope.
+
+(**
+ Allow the casual use of notations like nat * nat for explicit Type
+ declarations. Note that (nat * nat : Type) is NOT equivalent to
+ (nat * nat)%%type, whose inferred type is legacy type "Set".                **)
+Notation "T : 'Type'" := (CoqCast T%type Type) (only parsing) : core_scope.
+(**  Allow similarly Prop annotation for, e.g., rewrite multirules. **)
+Notation "P : 'Prop'" := (CoqCast P%type Prop) (only parsing) : core_scope.
+
+(**  Constants for abstract: and #[#: name #]# intro pattern  **)
+Definition abstract_lock := unit.
+Definition abstract_key := tt.
+
+Definition abstract (statement : Type) (id : nat) (lock : abstract_lock) :=
+  let: tt := lock in statement.
+
+Declare Scope ssr_scope.
+Notation "<hidden n >" := (abstract _ n _) : ssr_scope.
+Notation "T (* n *)" := (abstract T n abstract_key) : ssr_scope.
+Open Scope ssr_scope.
+
+Register abstract_lock as plugins.ssreflect.abstract_lock.
+Register abstract_key as plugins.ssreflect.abstract_key.
+Register abstract as plugins.ssreflect.abstract.
+
+(**  Constants for tactic-views  **)
+Inductive external_view : Type := tactic_view of Type.
+
+(**
+ Syntax for referring to canonical structures:
+      #[#the struct_type of proj_val by proj_fun#]#
+ This form denotes the Canonical instance s of the Structure type
+ struct_type whose proj_fun projection is proj_val, i.e., such that
+      proj_fun s = proj_val.
+ Typically proj_fun will be A record field accessors of struct_type, but
+ this need not be the case; it can be, for instance, a field of a record
+ type to which struct_type coerces; proj_val will likewise be coerced to
+ the return type of proj_fun. In all but the simplest cases, proj_fun
+ should be eta-expanded to allow for the insertion of implicit arguments.
+   In the common case where proj_fun itself is a coercion, the "by" part
+ can be omitted entirely; in this case it is inferred by casting s to the
+ inferred type of proj_val. Obviously the latter can be fixed by using an
+ explicit cast on proj_val, and it is highly recommended to do so when the
+ return type intended for proj_fun is "Type", as the type inferred for
+ proj_val may vary because of sort polymorphism (it could be Set or Prop).
+   Note when using the #[#the _ of _ #]# form to generate a substructure from a
+ telescopes-style canonical hierarchy (implementing inheritance with
+ coercions), one should always project or coerce the value to the BASE
+ structure, because Coq will only find a Canonical derived structure for
+ the Canonical base structure -- not for a base structure that is specific
+ to proj_value.                                                              **)
+
+Module TheCanonical.
+
+#[universes(template)]
+Variant put vT sT (v1 v2 : vT) (s : sT) := Put.
+
+Definition get vT sT v s (p : @put vT sT v v s) := let: Put _ _ _ := p in s.
+
+Definition get_by vT sT of sT -> vT := @get vT sT.
+
+End TheCanonical.
+
+Import TheCanonical. (* Note: no export. *)
+
+Local Arguments get_by _%type_scope _%type_scope _ _ _ _.
+
+Notation "[ 'the' sT 'of' v 'by' f ]" :=
+  (@get_by _ sT f _ _ ((fun v' (s : sT) => Put v' (f s) s) v _))
+  (only parsing) : form_scope.
+
+Notation "[ 'the' sT 'of' v ]" := (get ((fun s : sT => Put v (*coerce*) s s) _))
+  (only parsing) : form_scope.
+
+(**
+ The following are "format only" versions of the above notations.
+ We need to do this to prevent the formatter from being be thrown off by
+ application collapsing, coercion insertion and beta reduction in the right
+ hand side of the notations above.                                           **)
+
+Notation "[ 'the' sT 'of' v 'by' f ]" := (@get_by _ sT f v _ _)
+  (only printing) : form_scope.
+
+Notation "[ 'the' sT 'of' v ]" := (@get _ sT v _ _)
+  (only printing) : form_scope.
+
+(**
+ We would like to recognize
+Notation " #[# 'the' sT 'of' v : 'Type' #]#" := (@get Type sT v _ _)
+  (at level 0, format " #[# 'the'  sT   'of'  v  :  'Type' #]#") : form_scope.
+ **)
+
+(**
+ Helper notation for canonical structure inheritance support.
+ This is a workaround for the poor interaction between delta reduction and
+ canonical projections in Coq's unification algorithm, by which transparent
+ definitions hide canonical instances, i.e., in
+   Canonical a_type_struct := @Struct a_type ...
+   Definition my_type := a_type.
+ my_type doesn't effectively inherit the struct structure from a_type. Our
+ solution is to redeclare the instance as follows
+   Canonical my_type_struct := Eval hnf in #[#struct of my_type#]#.
+ The special notation #[#str of _ #]# must be defined for each Strucure "str"
+ with constructor "Str", typically as follows
+   Definition clone_str s :=
+      let: Str _ x y ... z := s return {type of Str for s} -> str in
+      fun k => k _ x y ... z.
+    Notation " #[# 'str' 'of' T 'for' s #]#" := (@clone_str s (@Str T))
+      (at level 0, format " #[# 'str'  'of'  T  'for'  s #]#") : form_scope.
+    Notation " #[# 'str' 'of' T #]#" := (repack_str (fun x => @Str T x))
+      (at level 0, format " #[# 'str'  'of'  T #]#") : form_scope.
+ The notation for the match return predicate is defined below; the eta
+ expansion in the second form serves both to distinguish it from the first
+ and to avoid the delta reduction problem.
+   There are several variations on the notation and the definition of the
+ the "clone" function, for telescopes, mixin classes, and join (multiple
+ inheritance) classes. We describe a different idiom for clones in ssrfun;
+ it uses phantom types (see below) and static unification; see fintype and
+ ssralg for examples.                                                        **)
+
+Definition argumentType T P & forall x : T, P x := T.
+Definition dependentReturnType T P & forall x : T, P x := P.
+Definition returnType aT rT & aT -> rT := rT.
+
+Notation "{ 'type' 'of' c 'for' s }" := (dependentReturnType c s) : type_scope.
+
+(**
+ A generic "phantom" type (actually, a unit type with a phantom parameter).
+ This type can be used for type definitions that require some Structure
+ on one of their parameters, to allow Coq to infer said structure so it
+ does not have to be supplied explicitly or via the " #[#the _ of _ #]#" notation
+ (the latter interacts poorly with other Notation).
+   The definition of a (co)inductive type with a parameter p : p_type, that
+ needs to use the operations of a structure
+  Structure p_str : Type := p_Str {p_repr :> p_type; p_op : p_repr -> ...}
+ should be given as
+  Inductive indt_type (p : p_str) := Indt ... .
+  Definition indt_of (p : p_str) & phantom p_type p := indt_type p.
+  Notation "{ 'indt' p }" := (indt_of (Phantom p)).
+  Definition indt p x y ... z : {indt p} := @Indt p x y ... z.
+  Notation " #[# 'indt' x y ... z #]#" := (indt x y ... z).
+ That is, the concrete type and its constructor should be shadowed by
+ definitions that use a phantom argument to infer and display the true
+ value of p (in practice, the "indt" constructor often performs additional
+ functions, like "locking" the representation -- see below).
+   We also define a simpler version ("phant" / "Phant") of phantom for the
+ common case where p_type is Type.                                           **)
+
+#[universes(template)]
+Variant phantom T (p : T) := Phantom.
+Arguments phantom : clear implicits.
+Arguments Phantom : clear implicits.
+#[universes(template)]
+Variant phant (p : Type) := Phant.
+
+(**  Internal tagging used by the implementation of the ssreflect elim.  **)
+
+Definition protect_term (A : Type) (x : A) : A := x.
+
+Register protect_term as plugins.ssreflect.protect_term.
+
+(**
+ The ssreflect idiom for a non-keyed pattern:
+  - unkeyed t will match any subterm that unifies with t, regardless of
+    whether it displays the same head symbol as t.
+  - unkeyed t a b will match any application of a term f unifying with t,
+    to two arguments unifying with with a and b, respectively, regardless of
+    apparent head symbols.
+  - unkeyed x where x is a variable will match any subterm with the same
+    type as x (when x would raise the 'indeterminate pattern' error).        **)
+
+Notation unkeyed x := (let flex := x in flex).
+
+(**  Ssreflect converse rewrite rule rule idiom.  **)
+Definition ssr_converse R (r : R) := (Logic.I, r).
+Notation "=^~ r" := (ssr_converse r) : form_scope.
+
+(**
+ Term tagging (user-level).
+ The ssreflect library uses four strengths of term tagging to restrict
+ convertibility during type checking:
+  nosimpl t simplifies to t EXCEPT in a definition; more precisely, given
+    Definition foo := nosimpl bar, foo (or foo t') will NOT be expanded by
+    the /= and //= switches unless it is in a forcing context (e.g., in
+    match foo t' with ... end, foo t' will be reduced if this allows the
+    match to be reduced). Note that nosimpl bar is simply notation for a
+    a term that beta-iota reduces to bar; hence rewrite /foo will replace
+    foo by bar, and rewrite -/foo will replace bar by foo.
+    CAVEAT: nosimpl should not be used inside a Section, because the end of
+    section "cooking" removes the iota redex.
+  locked t is provably equal to t, but is not convertible to t; 'locked'
+    provides support for selective rewriting, via the lock t : t = locked t
+    Lemma, and the ssreflect unlock tactic.
+  locked_with k t is equal but not convertible to t, much like locked t,
+    but supports explicit tagging with a value k : unit. This is used to
+    mitigate a flaw in the term comparison heuristic of the Coq kernel,
+    which treats all terms of the form locked t as equal and compares their
+    arguments recursively, leading to an exponential blowup of comparison.
+    For this reason locked_with should be used rather than locked when
+    defining ADT operations. The unlock tactic does not support locked_with
+    but the unlock rewrite rule does, via the unlockable interface.
+  we also use Module Type ascription to create truly opaque constants,
+    because simple expansion of constants to reveal an unreducible term
+    doubles the time complexity of a negative comparison. Such opaque
+    constants can be expanded generically with the unlock rewrite rule.
+    See the definition of card and subset in fintype for examples of this.   **)
+
+Notation nosimpl t := (let: tt := tt in t).
+
+Lemma master_key : unit. Proof. exact tt. Qed.
+Definition locked A := let: tt := master_key in fun x : A => x.
+
+Register master_key as plugins.ssreflect.master_key.
+Register locked as plugins.ssreflect.locked.
+
+Lemma lock A x : x = locked x :> A. Proof. unlock; reflexivity. Qed.
+
+(**  Needed for locked predicates, in particular for eqType's.  **)
+Lemma not_locked_false_eq_true : locked false <> true.
+Proof. unlock; discriminate. Qed.
+
+(**  The basic closing tactic "done".  **)
+Ltac done :=
+  trivial; hnf; intros; solve
+   [ do ![solve [trivial | apply: sym_equal; trivial]
+         | discriminate | contradiction | split]
+   | case not_locked_false_eq_true; assumption
+   | match goal with H : ~ _ |- _ => solve [case H; trivial] end ].
+
+(**  Quicker done tactic not including split, syntax: /0/  **)
+Ltac ssrdone0 :=
+  trivial; hnf; intros; solve
+   [ do ![solve [trivial | apply: sym_equal; trivial]
+         | discriminate | contradiction ]
+   | case not_locked_false_eq_true; assumption
+   | match goal with H : ~ _ |- _ => solve [case H; trivial] end ].
+
+(**  To unlock opaque constants.  **)
+#[universes(template)]
+Structure unlockable T v := Unlockable {unlocked : T; _ : unlocked = v}.
+Lemma unlock T x C : @unlocked T x C = x. Proof. by case: C. Qed.
+
+Notation "[ 'unlockable' 'of' C ]" :=
+  (@Unlockable _ _ C (unlock _)) : form_scope.
+
+Notation "[ 'unlockable' 'fun' C ]" :=
+  (@Unlockable _ (fun _ => _) C (unlock _)) : form_scope.
+
+(**  Generic keyed constant locking.  **)
+
+(**  The argument order ensures that k is always compared before T.  **)
+Definition locked_with k := let: tt := k in fun T x => x : T.
+
+(**
+ This can be used as a cheap alternative to cloning the unlockable instance
+ below, but with caution as unkeyed matching can be expensive.               **)
+Lemma locked_withE T k x : unkeyed (locked_with k x) = x :> T.
+Proof. by case: k. Qed.
+
+(**  Intensionaly, this instance will not apply to locked u.  **)
+Canonical locked_with_unlockable T k x :=
+  @Unlockable T x (locked_with k x) (locked_withE k x).
+
+(**  More accurate variant of unlock, and safer alternative to locked_withE. **)
+Lemma unlock_with T k x : unlocked (locked_with_unlockable k x) = x :> T.
+Proof. exact: unlock. Qed.
+
+(**  The internal lemmas for the have tactics.  **)
+
+Definition ssr_have Plemma Pgoal (step : Plemma) rest : Pgoal := rest step.
+Arguments ssr_have Plemma [Pgoal].
+
+Definition ssr_have_let Pgoal Plemma step
+  (rest : let x : Plemma := step in Pgoal) : Pgoal := rest.
+Arguments ssr_have_let [Pgoal].
+
+Register ssr_have as plugins.ssreflect.ssr_have.
+Register ssr_have_let as plugins.ssreflect.ssr_have_let.
+
+Definition ssr_suff Plemma Pgoal step (rest : Plemma) : Pgoal := step rest.
+Arguments ssr_suff Plemma [Pgoal].
+
+Definition ssr_wlog := ssr_suff.
+Arguments ssr_wlog Plemma [Pgoal].
+
+Register ssr_suff as plugins.ssreflect.ssr_suff.
+Register ssr_wlog as plugins.ssreflect.ssr_wlog.
+
+(**  Internal N-ary congruence lemmas for the congr tactic.  **)
+
+Fixpoint nary_congruence_statement (n : nat)
+         : (forall B, (B -> B -> Prop) -> Prop) -> Prop :=
+  match n with
+  | O => fun k => forall B, k B (fun x1 x2 : B => x1 = x2)
+  | S n' =>
+    let k' A B e (f1 f2 : A -> B) :=
+      forall x1 x2, x1 = x2 -> (e (f1 x1) (f2 x2) : Prop) in
+    fun k => forall A, nary_congruence_statement n' (fun B e => k _ (k' A B e))
+  end.
+
+Lemma nary_congruence n (k := fun B e => forall y : B, (e y y : Prop)) :
+  nary_congruence_statement n k.
+Proof.
+have: k _ _ := _; rewrite {1}/k.
+elim: n k  => [|n IHn] k k_P /= A; first exact: k_P.
+by apply: IHn => B e He; apply: k_P => f x1 x2 <-.
+Qed.
+
+Lemma ssr_congr_arrow Plemma Pgoal : Plemma = Pgoal -> Plemma -> Pgoal.
+Proof. by move->. Qed.
+Arguments ssr_congr_arrow : clear implicits.
+
+Register nary_congruence as plugins.ssreflect.nary_congruence.
+Register ssr_congr_arrow as plugins.ssreflect.ssr_congr_arrow.
+
+(**  View lemmas that don't use reflection.  **)
+
+Section ApplyIff.
+
+Variables P Q : Prop.
+Hypothesis eqPQ : P <-> Q.
+
+Lemma iffLR : P -> Q. Proof. by case: eqPQ. Qed.
+Lemma iffRL : Q -> P. Proof. by case: eqPQ. Qed.
+
+Lemma iffLRn : ~P -> ~Q. Proof. by move=> nP tQ; case: nP; case: eqPQ tQ. Qed.
+Lemma iffRLn : ~Q -> ~P. Proof. by move=> nQ tP; case: nQ; case: eqPQ tP. Qed.
+
+End ApplyIff.
+
+Hint View for move/ iffLRn|2 iffRLn|2 iffLR|2 iffRL|2.
+Hint View for apply/ iffRLn|2 iffLRn|2 iffRL|2 iffLR|2.
+
+(**
+ To focus non-ssreflect tactics on a subterm, eg vm_compute.
+ Usage:
+   elim/abstract_context: (pattern) => G defG.
+   vm_compute; rewrite {}defG {G}.
+ Note that vm_cast are not stored in the proof term
+ for reductions occurring in the context, hence
+   set here := pattern; vm_compute in (value of here)
+ blows up at Qed time.                                        **)
+Lemma abstract_context T (P : T -> Type) x :
+  (forall Q, Q = P -> Q x) -> P x.
+Proof. by move=> /(_ P); apply. Qed.
+
+(*****************************************************************************)
+(* Material for under/over (to rewrite under binders using "context lemmas") *)
+
+Require Export ssrunder.
+
+Hint Extern 0 (@Under_rel.Over_rel _ _ _ _) =>
+  solve [ apply: Under_rel.over_rel_done ] : core.
+Hint Resolve Under_rel.over_rel_done : core.
+
+Register Under_rel.Under_rel as plugins.ssreflect.Under_rel.
+Register Under_rel.Under_rel_from_rel as plugins.ssreflect.Under_rel_from_rel.
+
+(** Closing rewrite rule *)
+Definition over := over_rel.
+
+(** Closing tactic *)
+Ltac over :=
+  by [ apply: Under_rel.under_rel_done
+     | rewrite over
+     ].
+
+(** Convenience rewrite rule to unprotect evars, e.g., to instantiate
+    them in another way than with reflexivity. *)
+Definition UnderE := Under_relE.
+
+(*****************************************************************************)
+
+(** An interface for non-Prop types; used to avoid improper instantiation
+    of polymorphic lemmas with on-demand implicits when they are used as views.
+    For example: Some_inj {T} : forall x y : T, Some x = Some y -> x = y.
+    Using move/Some_inj on a goal of the form Some n = Some 0 will fail:
+    SSReflect will interpret the view as @Some_inj ?T _top_assumption_
+    since this is the well-typed application of the view with the minimal
+    number of inserted evars (taking ?T := Some n = Some 0), and then will
+    later complain that it cannot erase _top_assumption_ after having
+    abstracted the viewed assumption. Making x and y maximal implicits
+    would avoid this and force the intended @Some_inj nat x y _top_assumption_
+    interpretation, but is undesirable as it makes it harder to use Some_inj
+    with the many SSReflect and MathComp lemmas that have an injectivity
+    premise. Specifying {T : nonPropType} solves this more elegantly, as then
+    (?T : Type) no longer unifies with (Some n = Some 0), which has sort Prop.
+ **)
+
+Module NonPropType.
+
+(** Implementation notes:
+ We rely on three interface Structures:
+  - test_of r, the middle structure, performs the actual check: it has two
+    canonical instances whose 'condition' projection are maybeProj (?P : Prop)
+    and tt, and which set r := true and r := false, respectively. Unifying
+    condition (?t : test_of ?r) with maybeProj T will thus set ?r to true if
+    T is in Prop as the test_Prop T instance will apply, and otherwise simplify
+    maybeProp T to tt and use the test_negative instance and set ?r to false.
+  - call_of c r sets up a call to test_of on condition c with expected result r.
+    It has a default instance for its 'callee' projection to Type, which
+    sets c := maybeProj T and r := false when unifying with a type T.
+  - type is a telescope on call_of c r, which checks that unifying test_of ?r1
+    with c indeed sets ?r1 := r; the type structure bundles the 'test' instance
+    and its 'result' value along with its call_of c r projection. The default
+    instance essentially provides eta-expansion for 'type'. This is only
+    essential for the first 'result' projection to bool; using the instance
+    for other projection merely avoids spurious delta expansions that would
+    spoil the notProp T notation.
+ In detail, unifying T =~= ?S with ?S : nonPropType, i.e.,
+  (1)  T =~= @callee (@condition (result ?S) (test ?S)) (result ?S) (frame ?S)
+ first uses the default call instance with ?T := T to reduce (1) to
+  (2a) @condition (result ?S) (test ?S) =~= maybeProp T
+  (3)                         result ?S =~= false
+  (4)                          frame ?S =~= call T
+ along with some trivial universe-related checks which are irrelevant here.
+   Then the unification tries to use the test_Prop instance to reduce (2a) to
+  (6a)                        result ?S =~= true
+  (7a)                               ?P =~= T with ?P : Prop
+  (8a)                          test ?S =~= test_Prop ?P
+ Now the default 'check' instance with ?result := true resolves (6a) as
+  (9a)                               ?S := @check true ?test ?frame
+ Then (7a) can be solved precisely if T has sort at most (hence exactly) Prop,
+ and then (8a) is solved by the check instance, yielding ?test := test_Prop T,
+ and completing the solution of (2a), and _committing_ to it. But now (3) is
+ inconsistent with (9a), and this makes the entire problem (1) fails.
+   If on the othe hand T does not have sort Prop then (7a) fails and the
+ unification resorts to delta expanding (2a), which gives
+  (2b) @condition (result ?S) (test ?S) =~= tt
+ which is then reduced, using the test_negative instance, to
+  (6b)                        result ?S =~= false
+  (8b)                          test ?S =~= test_negative
+ Both are solved using the check default instance, as in the (2a) branch, giving
+  (9b)                               ?S := @check false test_negative ?frame
+ Then (3) and (4) are similarly soved using check, giving the final assignment
+  (9)                                ?S := notProp T
+ Observe that we _must_ perform the actual test unification on the arguments
+ of the initial canonical instance, and not on the instance itself as we do
+ in mathcomp/matrix and mathcomp/vector, because we want the unification to
+ fail when T has sort Prop. If both the test_of _and_ the result check
+ unifications were done as part of the structure telescope then the latter
+ would be a sub-problem of the former, and thus failing the check would merely
+ make the test_of unification backtrack and delta-expand and we would not get
+ failure.
+ **)
+
+Structure call_of (condition : unit) (result : bool) := Call {callee : Type}.
+Definition maybeProp (T : Type) := tt.
+Definition call T := Call (maybeProp T) false T.
+
+Structure test_of (result : bool) := Test {condition :> unit}.
+Definition test_Prop (P : Prop) := Test true (maybeProp P).
+Definition test_negative := Test false tt.
+
+Structure type :=
+  Check {result : bool; test : test_of result; frame : call_of test result}.
+Definition check result test frame := @Check result test frame.
+
+Module Exports.
+Canonical call.
+Canonical test_Prop.
+Canonical test_negative.
+Canonical check.
+Notation nonPropType := type.
+Coercion callee : call_of >-> Sortclass.
+Coercion frame : type >-> call_of.
+Notation notProp T := (@check false test_negative (call T)).
+End Exports.
+
+End NonPropType.
+Export NonPropType.Exports.
